@prefix : <https://johnson14988.github.io/Source/docs/ontology/program#> .
@prefix owl: <http://www.w3.org/2002/07/owl#> .
@prefix rdf: <http://www.w3.org/1999/02/22-rdf-syntax-ns#> .
@prefix xml: <http://www.w3.org/XML/1998/namespace> .
@prefix xsd: <http://www.w3.org/2001/XMLSchema#> .
@prefix rdfs: <http://www.w3.org/2000/01/rdf-schema#> .
@prefix program: <https://johnson14988.github.io/Source/docs/ontology/program#> .
@base <https://johnson14988.github.io/Source/docs/ontology/program> .

<https://johnson14988.github.io/Source/docs/ontology/program> rdf:type owl:Ontology .

#################################################################
#    Classes
#################################################################

###  https://johnson14988.github.io/Source/docs/ontology/program#Affective
program:Affective rdf:type owl:Class ;
                  rdfs:subClassOf program:Goal .


###  https://johnson14988.github.io/Source/docs/ontology/program#Analyze
program:Analyze rdf:type owl:Class ;
                rdfs:subClassOf program:Cognitive ;
                rdfs:comment "Draw connections among ideas: differentiate, organize, relate, compare, contrast, distinguish, examine, experiment, question, test." .


###  https://johnson14988.github.io/Source/docs/ontology/program#Apply
program:Apply rdf:type owl:Class ;
              rdfs:subClassOf program:Cognitive ;
              rdfs:comment "Use information in new situations: execute, implement, solve, use, demonstrate, interpret, operate, schedule, sketch." .


###  https://johnson14988.github.io/Source/docs/ontology/program#Cognitive
program:Cognitive rdf:type owl:Class ;
                  rdfs:subClassOf program:Goal .


###  https://johnson14988.github.io/Source/docs/ontology/program#Create
program:Create rdf:type owl:Class ;
               rdfs:subClassOf program:Cognitive ;
               rdfs:comment "Produce new or original work: design, assemble, construct, develop, formulate, investigate, write, present." .


###  https://johnson14988.github.io/Source/docs/ontology/program#Evaluate
program:Evaluate rdf:type owl:Class ;
                 rdfs:subClassOf program:Cognitive ;
                 rdfs:comment "Justify a stand or decision: appraise, argue, defend, judge, select, support, value, critique, weigh." .


###  https://johnson14988.github.io/Source/docs/ontology/program#Goal
program:Goal rdf:type owl:Class .


###  https://johnson14988.github.io/Source/docs/ontology/program#Psychomotor
program:Psychomotor rdf:type owl:Class ;
                    rdfs:subClassOf program:Goal .


###  https://johnson14988.github.io/Source/docs/ontology/program#Remember
program:Remember rdf:type owl:Class ;
                 rdfs:subClassOf program:Cognitive ;
                 rdfs:comment "Recall facts and basic concepts: define, duplicate, list, memorize, repeat, state." .


###  https://johnson14988.github.io/Source/docs/ontology/program#Task
program:Task rdf:type owl:Class .


###  https://johnson14988.github.io/Source/docs/ontology/program#Understand
program:Understand rdf:type owl:Class ;
                   rdfs:subClassOf program:Cognitive ;
                   rdfs:comment "Explain ideas or concepts: classify, describe, discuss, explain, identify, locate, recognize, report, select, translate." .


###  Generated by the OWL API (version 4.5.29.2024-05-13T12:11:03Z) https://github.com/owlcs/owlapi
